rupicola/stlc_v2/ExpRel.fst
@@ -11,26 +11,28 @@ let fs_empty : fs_env empty =
     #(fun x -> get_Type (Some?.v (empty x)))
     (fun _ -> assert False)
 
-let get_v #g fs_s x = fs_s x
-
-let fs_extend #g fs_s #t fs_v =
+let fs_stack #g fs_s #t fs_v =
   on_dom
     (x:var{Some? ((extend t g) x)})
     #(fun x -> get_Type (Some?.v ((extend t g) x)))
     (fun y ->
       if y = 0 then fs_v else fs_s (y-1))
 
-let fs_shrink #t #g fs_s =
+let fs_hd #g fs_s = fs_s 0
+
+let fs_tail #t #g fs_s =
   on_dom
     (x:var{Some? (g x)})
     #(fun x -> get_Type (Some?.v (g x)))
     (fun y -> fs_s (y+1))
 
+let get_v #g fs_s x = fs_s x
+
 let lem_fs_extend fs_s v = ()
 let lem_fs_shrink fs_s = ()
 
 let shrink_extend_inverse #g fs_s #t v =
-  let fs_s' : fs_env g = fs_shrink (fs_extend fs_s v) in
+  let fs_s' : fs_env g = fs_tail (fs_stack fs_s v) in
   assert (forall x. fs_s' x == fs_s x);
   assert (feq fs_s' fs_s);
   extensionality (x:var{Some? (g x)}) (fun x -> get_Type (Some?.v (g x))) fs_s' fs_s;
